theories/L2k_noCnstrParams/toplevel.v
@@ -4,7 +4,6 @@ Require Import L2k.term.
 Require Import Common.Common Common.compM Common.Pipeline_utils.
 From ExtLib Require Import Monads.
 
-
 Require Import Common.Common Common.classes Common.Pipeline_utils Common.compM.
 From ExtLib Require Import Monads.
 From MetaCoq.Template Require Import utils Typing.
@@ -35,10 +34,7 @@ Definition compile_L1g : CertiCoqTrans (global_context * term) (Program Term) :=
  *)
 
  Definition wf_program (p : Ast.Env.program) := 
-  ∥ ∑ T, @Typing.typing 
-    config.extraction_checker_flags
-    (Ast.Env.empty_ext p.1)
-    [] p.2 T ∥.
+  ∥ ∑ T, @Typing.typing config.extraction_checker_flags (Ast.Env.empty_ext p.1) [] p.2 T ∥.
 
 Definition template_bigstep (p : Ast.Env.program) (v : Ast.term) : Prop :=
   ∥ Template.WcbvEval.eval p.1 p.2 v ∥.
@@ -50,7 +46,7 @@ Definition template_bigstep (p : Ast.Env.program) (v : Ast.term) : Prop :=
 
 Import MonadNotation.
 
-Instance L2k_Lang : Lang (Program L2k.compile.Term) :=
+#[export] Instance L2k_Lang : Lang (Program L2k.compile.Term) :=
   { Value := Term;
     TermWf := fun P => L2k.program.crctTerm (AstCommon.env P) 0 (main P);
     BigStep := fun s sv => WcbvEval (env s) (main s) sv
